Rework argument parsing, add --tight-bounds-mul-by
The `--tight-bounds-mul-by` argument allows us to specify the tight
bounds multiplier manually.

Closes #800
Closes #796 (actually, this had already been implemented, though we now
use it for curve25519)
Closes #755 (machine_wordsize is now owned by the binary as a whole)

Note that the last of these necessitates moving machine_wordsize to come
right after curve_description.  Invoking the binaries in the old way may
result in them hanging for a long time while they try to compute
representations for, say, lists of 2^255-19 5-bit-limbs for the "prime"
64.

We now use a structured language to describe the command line arguments,
based on OCaml's Arg module interface.  The error and help messages are
now perhaps a tiny bit worse, but it should now be moderately easier to
add new optional command line arguments.

Note that named arguments now use spaces rather than equals signs to
pass values.

The old usage message:
```
USAGE: ./src/ExtractionOCaml/unsaturated_solinas [--lang=LANGUAGE] [--static] [--internal-static] [--no-wide-int] [--widen-carry] [--widen-bytes] [--no-select] [--split-multiret] [--no-primitives] [--cmovznz-by-mul] curve_description n s-c machine_wordsize [function_to_synthesize*]
Got 0 arguments.

  LANGUAGE                The output language code should be emitted in.  Defaults to C if no language is given.  Case-sensitive.
                            Valid options are: C, Rust, Go, Java
  --static                Declare the functions as static, i.e., local to the file.
  --internal-static       Declare internal functions as static, i.e., local to the file.
  --no-wide-int           Don't use integers wider than the bitwidth.
  --widen-carry           Widen carry bit integer types to either the byte type, or to the full bitwidth if --widen-bytes is also passed.
  --widen-bytes           Widen byte types to the full bitwidth.
  --no-select             Use expressions that don't require cmov.
  --split-multiret        Don't allow instructions to return two results. This should always be set for bedrock2.
  --no-primitives         Suppress the generation of the bodies of primitive operations such as addcarryx, subborrowx, cmovznz, mulx, etc.
  --cmovznz-by-mul        Use an alternative implementation of cmovznz using multiplication rather than bitwise-and with -1.
  curve_description       A string which will be prefixed to every function name generated
  n                       The number of limbs, or the literal '(auto)' or '(autoN)' for a non-negative number N, to automatically guess the number of limbs
  s-c                     The prime, which must be expressed as a difference of a power of two and a small field element (e.g., '2^255 - 19', '2^448 - 2^224 - 1')
  machine_wordsize        The machine bitwidth (e.g., 32 or 64)
  function_to_synthesize  A space-separated list of functions that should be synthesized.  If no functions are given, all functions are synthesized.
                            Valid options are carry_mul, carry_square, carry, add, sub, opp, selectznz, to_bytes, from_bytes, or 'carry_scmul' followed by a decimal literal

Fatal error: exception Failure("Synthesis failed")
```

The new usage message:
```
./src/ExtractionOCaml/unsaturated_solinas: option 'curve_description' needs an argument.

USAGE: ./src/ExtractionOCaml/unsaturated_solinas [OPTS...] curve_description machine_wordsize n s-c [function_to_synthesize...]

  --lang {C|Rust|Go|Java}  The output language code should be emitted in.  Defaults to C if no language is given.  Case-sensitive.
  --static                 Declare the functions as static, i.e., local to the file.
  --internal-static        Declare internal functions as static, i.e., local to the file.
  --no-wide-int            Don't use integers wider than the bitwidth.
  --widen-carry            Widen carry bit integer types to either the byte type, or to the full bitwidth if --widen-bytes is also passed.
  --widen-bytes            Widen byte types to the full bitwidth.
  --no-select              Use expressions that don't require cmov.
  --split-multiret         Don't allow instructions to return two results. This should always be set for bedrock2.
  --no-primitives          Suppress the generation of the bodies of primitive operations such as addcarryx, subborrowx, cmovznz, mulx, etc.
  --cmovznz-by-mul         Use an alternative implementation of cmovznz using multiplication rather than bitwise-and with -1.
  --only-signed            Only allow signed integer types.
  --tight-bounds-mul-by    The (improper) fraction by which the (tight) bounds of each limb are scaled
  -h, --help               Display this list of options
  curve_description        A string which will be prefixed to every function name generated
  machine_wordsize         The machine bitwidth (e.g., 32 or 64)
  n                        The number of limbs, or the literal '(auto)' or '(autoN)' for a non-negative number N, to automatically guess the number of limbs
  s-c                      The prime, which must be expressed as a difference of a power of two and a small field element (e.g., '2^255 - 19', '2^448 - 2^224 - 1')
  function_to_synthesize   A space-separated list of functions that should be synthesized.  If no functions are given, all functions are synthesized.
                           Valid options are carry_mul, carry_square, carry, add, sub, opp, selectznz, to_bytes, from_bytes, or 'carry_scmul' followed by a decimal literal.

Fatal error: exception Failure("Synthesis failed")
```

src/Util/Arg.v
@@ -1,5 +1,6 @@
 (** Coq version of OCaml's Arg module *)
 Require Import Coq.Lists.List.
+Require Import Coq.Strings.Ascii.
 Require Import Coq.Strings.String.
 Require Import Coq.ZArith.ZArith.
 Require Import Coq.Strings.OctalString.
@@ -9,6 +10,7 @@ Require Import Crypto.Util.Strings.Ascii.
 Require Import Crypto.Util.Strings.String.
 Require Import Crypto.Util.Strings.Decimal.
 Require Import Crypto.Util.Strings.Show.
+Require Import Crypto.Util.ListUtil.
 Require Import Crypto.Util.ErrorT.
 Require Import Crypto.Util.Option.
 Require Import Crypto.Util.Notations.
@@ -28,7 +30,8 @@ Inductive spec :=
 | Nat (b : list base_system)
 | Tuple (ls : list spec)
 | Symbol (syms : list string)
-| Custom (dataT : Type) (parse : string -> option dataT) (expected_descr : string)
+| CustomSymbol {dataT : Type} (syms : list (string * dataT))
+| Custom {dataT : Type} (parse : string -> option dataT) (expected_descr : string)
 .
 
 Inductive key := long_key (_ : string) | short_key (_ : string).
@@ -36,6 +39,11 @@ Definition doc := list string.
 Definition usage_msg := list string.
 
 Local Notation type_of_list l ls := (List.fold_left (fun a b : Type => prod a b) ls l).
+Local Notation type_of_list' ls
+  := match ls return Type with
+     | [] => unit
+     | l :: ls' => type_of_list l ls'
+     end.
 
 Fixpoint spec_data (s : spec) : Type
   := match s with
@@ -47,6 +55,7 @@ Fixpoint spec_data (s : spec) : Type
      | Tuple nil => unit
      | Tuple (l :: ls) => type_of_list (spec_data l) (List.map spec_data ls)
      | Symbol syms => string
+     | CustomSymbol dataT syms => dataT
      | Custom dataT parse err_msg => dataT
      end.
 
@@ -58,17 +67,67 @@ Definition opt_spec_data (opt : bool) (s : spec) : Type
   := if opt then option (spec_data s) else spec_data s.
 
 Definition keyed_spec_list_data (s : list (list key * spec * doc)) : Type
-  := match s with
-     | nil => unit
-     | (_, s, _) :: ss
-       => type_of_list (spec_data_with_key s) (List.map (fun '(_, s, _) => spec_data_with_key s) ss)
-     end.
+  := type_of_list' (List.map (fun '(_, s, _) => spec_data_with_key s) s).
 
 Definition spec_list_data (opt : bool) (s : list (string * spec * doc)) : Type
-  := match s with
-     | nil => unit
-     | (_, s, _) :: ss
-       => type_of_list (opt_spec_data opt s) (List.map (fun '(_, s, _) => opt_spec_data opt s) ss)
+  := type_of_list' (List.map (fun '(_, s, _) => opt_spec_data opt s) s).
+
+
+Fixpoint update_type_of_list (T1 T2 : Type) Ts (f : T1 -> T2) {struct Ts}
+  : type_of_list T1 Ts -> type_of_list T2 Ts
+  := match Ts return type_of_list T1 Ts -> type_of_list T2 Ts with
+     | nil => f
+     | cons T Ts
+       => @update_type_of_list _ _ Ts (fun '(t1, t) => (f t1, t))
+     end.
+
+Fixpoint update_type_of_list2 (T1 T2 T : Type) Ts {struct Ts}
+  : (type_of_list T1 Ts -> type_of_list T2 Ts) -> type_of_list (T * T1)%type Ts -> type_of_list (T * T2)%type Ts
+  := match Ts return (type_of_list T1 Ts -> type_of_list T2 Ts) -> type_of_list (T * T1)%type Ts -> type_of_list (T * T2)%type Ts with
+     | nil => fun f '(t, t1) => (t, f t1)
+     | cons T' Ts
+       => fun f v
+          => let v := @update_type_of_list
+                        _ _ Ts (fun '(a, b, c) => (a, (b, c)))
+                        v in
+             @update_type_of_list
+               _ _ Ts (fun '(a, (b, c)) => (a, b, c))
+               (@update_type_of_list2 _ _ _ Ts f v)
+     end.
+
+Definition cons_type_of_list {x x' xs} (v : x)
+  : type_of_list x' xs -> type_of_list x (x' :: xs)
+  := update_type_of_list _ _ _ (@pair _ _ v).
+
+Definition cons_type_of_list' {x xs} (v : x)
+  : type_of_list' xs -> type_of_list x xs
+  := match xs with
+     | [] => fun _ => v
+     | _ :: _ => @cons_type_of_list _ _ _ v
+     end.
+
+Fixpoint uncons_type_of_list {l ls}
+  : type_of_list l ls -> l * type_of_list' ls
+  := match ls return type_of_list l ls -> l * type_of_list' ls with
+     | [] => fun v => (v, tt)
+     | l' :: ls
+       => fun v
+          => let '(v, v', vs) := @uncons_type_of_list (l * l')%type ls v in
+             (v, cons_type_of_list' v' vs)
+     end.
+
+Fixpoint split_type_of_list_' {l1 ls1 ls2} {struct ls1}
+  : type_of_list l1 (ls1 ++ ls2) -> type_of_list l1 ls1 * type_of_list' ls2
+  := match ls1 with
+     | [] => uncons_type_of_list
+     | l1' :: ls1 => @split_type_of_list_' (l1 * l1')%type ls1 ls2
+     end.
+
+Definition split_type_of_list' {ls1 ls2}
+  : type_of_list' (ls1 ++ ls2) -> type_of_list' ls1 * type_of_list' ls2
+  := match ls1 with
+     | [] => @pair _ _ tt
+     | _ :: _ => split_type_of_list_'
      end.
 
 Local Definition make_symlist prefix sep suffix l
@@ -90,33 +149,35 @@ Local Definition print_key_list (k : list key) : string
      | k => String.concat ", " (List.map print_key k)
      end.
 
-Local Definition print_spec : (list key + string) * spec * doc -> list string
+Local Definition print_spec_parts : (list key + string) * spec * doc -> string * list string
   := fun '(k, s, d)
      => if Nat.ltb 0 (doc_length d)
-        then (["  "
+        then (("  "
                  ++ (match k with
                      | inl k => print_key_list k
                      | inr k => k
                      end) ++ " "
                  ++ (match s with
                      | Symbol syms => make_symlist "{" "|" "}" syms
+                     | CustomSymbol _ syms => make_symlist "{" "|" "}" (List.map (@fst _ _) syms)
                      | _ => ""
-                     end)
-                 ++ (hd "" d)
-                 ++ (if Nat.eqb (List.length (tl d)) 0 then String.NewLine else "")]%string)
-               ++ tl d ++ (if Nat.eqb (List.length (tl d)) 0 then nil else [String.NewLine])
-        else nil.
+                     end))%string,
+              ([hd "" d])
+                ++ tl d
+                ++ (if Nat.eqb (List.length (tl d)) 0 then nil else [""]))
+        else ("", nil).
 
 Definition print_spec_short (k : string) (s : spec) : string
   := match s with
      | Symbol syms => make_symlist "{" "|" "}" syms
+     | CustomSymbol _ syms => make_symlist "{" "|" "}" (List.map (@fst _ _) syms)
      | _ => k
      end.
 
 Local Definition help_specs : list (list key * spec * doc)
   := [([short_key "h"; long_key "help"],
        Unit,
-       [" Display this list of options"])].
+       ["Display this list of options"])].
 
 Definition arg_matches_key (arg : string) (k : key) : bool
   := (arg =? print_key k)%string.
@@ -176,9 +237,11 @@ Inductive parse_error :=
 | help (prog_name : string)
 | missing (prog_name : string) (opt_name : string)
 | wrong (prog_name : string) (opt_name : string) (got : string) (expected : string)
+| no_keyed_arg (prog_name : string) (bad_args : list string)
 | missing_prog_name
 | too_many_args (prog_name : string) (remaining : list string)
-| out_of_fuel (prog_name : string).
+| out_of_fuel (prog_name : string)
+| internal_error (prog_name : string) (msg : string).
 
 Definition parse_result T := ErrorT parse_error T.
 
@@ -235,11 +298,17 @@ Fixpoint parse_args_via_spec (s : spec) (argv : list string)
        => if List.existsb (fun s => arg =? s)%string syms
           then Success (arg, argv)
           else Error (wrong arg ("one of: " ++ (make_symlist "" " " "" syms))%string)
+     | CustomSymbol dataT syms, arg::argv
+       => match List.find (fun '(s, v) => arg =? s)%string syms with
+          | Some (s, v) => Success (v, argv)
+          | None => Error (wrong arg ("one of: " ++ (make_symlist "" " " "" (List.map (@fst _ _) syms)))%string)
+          end
      | Bool, nil
      | String, nil
      | Int _, nil
      | Nat _, nil
      | Symbol _, nil
+     | CustomSymbol _ _, nil
      | Custom _ _ _, nil
        => Error missing
      end%error.
@@ -250,13 +319,33 @@ Record arg_spec :=
     anon_opt_args : list (string * spec * doc);
     anon_opt_repeated_arg : option (string * spec * doc) }.
 
-Definition usage_string : arg_spec -> usage_msg -> list string
+Inductive ShouldBlockIndent := NoIndent | ArbitraryIndent | IndentUpTo (n : nat).
+Existing Class ShouldBlockIndent.
+
+Local Definition spaces (n : nat) : string
+  := String.string_of_list_ascii (List.repeat " "%char n).
+
+Local Definition maybe_block_indent {should_block_indent : ShouldBlockIndent} (indent : nat) (lhs : string) (rhs : list string)
+  := let lhs := (lhs ++ "  ")%string in
+     let indent := match should_block_indent with
+                   | NoIndent => spaces (String.length lhs)
+                   | ArbitraryIndent => spaces indent
+                   | IndentUpTo n => spaces (Nat.min indent n)
+                   end in
+     ((lhs ++ String.substring 0 (String.length indent - String.length lhs) indent ++ hd "" rhs)%string)
+       :: List.map (fun s => indent ++ s)%string (tl rhs).
+
+Definition usage_string {should_block_indent : ShouldBlockIndent} : arg_spec -> usage_msg -> list string
   := fun specs err
      => err
           ++ [String.NewLine]
-          ++ List.flat_map (fun '(k, s, d) => print_spec (inl k, s, d)) (specs.(named_args) ++ help_specs)
-          ++ List.flat_map (fun '(k, s, d) => print_spec (inr k, s, d)) (specs.(anon_args) ++ specs.(anon_opt_args) ++ match specs.(anon_opt_repeated_arg) with Some v => [v] | None => nil end).
-
+          ++ (let spec_parts
+                  := ((List.map (fun '(k, s, d) => print_spec_parts (inl k, s, d)) (specs.(named_args) ++ help_specs))
+                        ++ (List.map (fun '(k, s, d) => print_spec_parts (inr k, s, d)) (specs.(anon_args) ++ specs.(anon_opt_args) ++ match specs.(anon_opt_repeated_arg) with Some v => [v] | None => nil end))) in
+              let max_length := List.fold_right Nat.max O (List.map String.length (List.map (@fst _ _) spec_parts)) in
+              List.flat_map
+                (fun '(lhs, rhs) => maybe_block_indent (2 + max_length) lhs rhs)
+                spec_parts).
 
 Definition arg_spec_results (s : arg_spec)
   := (keyed_spec_list_data s.(named_args) * spec_list_data false s.(anon_args) * spec_list_data true s.(anon_opt_args) * (match s.(anon_opt_repeated_arg) with None => unit | Some (k, s, d) => list (spec_data s) end))%type.
@@ -268,33 +357,12 @@ Definition consume_one_named_arg
          (missing : parse_error)
          (wrong : string (* got *) -> string (* expected *) -> parse_error)
   : parse_result (option ((spec_data_with_key (snd (fst named_arg)) -> spec_data_with_key (snd (fst named_arg)))
-                          * list string (* remaining *) * list string (* accumulated positional args *)))
+                          * list string (* remaining *)))
   := (if arg_matches_key_list arg (fst (fst named_arg))
-      then res <- parse_args_via_spec (snd (fst named_arg)) argv missing wrong;
-             Success (Some ((fun data_so_far => data_so_far ++ [(arg, fst res)]), snd res, nil))
+      then (res <- parse_args_via_spec (snd (fst named_arg)) argv missing wrong;
+           Success (Some ((fun data_so_far => data_so_far ++ [(arg, fst res)]), snd res)))
       else Success None)%error.
 
-Fixpoint update_type_of_list (T1 T2 : Type) Ts (f : T1 -> T2) {struct Ts}
-  : type_of_list T1 Ts -> type_of_list T2 Ts
-  := match Ts return type_of_list T1 Ts -> type_of_list T2 Ts with
-     | nil => f
-     | cons T Ts
-       => @update_type_of_list _ _ Ts (fun '(t1, t) => (f t1, t))
-     end.
-
-Fixpoint update_type_of_list2 (T1 T2 T : Type) Ts {struct Ts}
-  : (type_of_list T1 Ts -> type_of_list T2 Ts) -> type_of_list (T * T1)%type Ts -> type_of_list (T * T2)%type Ts
-  := match Ts return (type_of_list T1 Ts -> type_of_list T2 Ts) -> type_of_list (T * T1)%type Ts -> type_of_list (T * T2)%type Ts with
-     | nil => fun f '(t, t1) => (t, f t1)
-     | cons T' Ts
-       => fun f v
-          => let v := @update_type_of_list
-                        _ _ Ts (fun '(a, b, c) => (a, (b, c)))
-                        v in
-             @update_type_of_list
-               _ _ Ts (fun '(a, (b, c)) => (a, b, c))
-               (@update_type_of_list2 _ _ _ Ts f v)
-     end.
 
 Fixpoint consume_named_arg
          (arg : string)
@@ -303,18 +371,18 @@ Fixpoint consume_named_arg
          (missing : string (* key *) -> parse_error)
          (wrong : string (* key *) -> string (* got *) -> string (* expected *) -> parse_error)
          {struct named_args}
-  : parse_result ((keyed_spec_list_data named_args -> keyed_spec_list_data named_args) * list string (* remaining *) * list string (* accumulated positional args *))
-  := (match named_args return parse_result ((keyed_spec_list_data named_args -> keyed_spec_list_data named_args) * list string (* remaining *) * list string (* accumulated positional args *))
+  : parse_result ((keyed_spec_list_data named_args -> keyed_spec_list_data named_args) * list string (* remaining *))
+  := (match named_args return parse_result ((keyed_spec_list_data named_args -> keyed_spec_list_data named_args) * list string (* remaining *))
       with
-      | nil => Success (fun data_so_far => data_so_far, nil, arg::argv)
+      | nil => Success (fun data_so_far => data_so_far, arg::argv)
       | (k, s, d) :: named_args
         => (lv <- consume_one_named_arg arg argv (k, s, d) (missing arg) (wrong arg);
               match lv with
-              | Some (upd, argv, pos_args)
-                => Success (update_type_of_list _ _ _ upd, argv, pos_args)
+              | Some (upd, argv)
+                => Success (update_type_of_list _ _ _ upd, argv)
               | None
                 => (rec <- @consume_named_arg arg argv named_args missing wrong;
-                      let '(upd, argv, pos_args) := rec in
+                      let '(upd, argv) := rec in
                       Success (match named_args
                                      return (keyed_spec_list_data named_args -> keyed_spec_list_data named_args) ->
                                             type_of_list (spec_data_with_key s) (List.map (fun '(_, s0, _) => spec_data_with_key s0) named_args) ->
@@ -323,8 +391,7 @@ Fixpoint consume_named_arg
                                | nil => fun _ x => x
                                | cons (k', s', d') xs => update_type_of_list2 _ _ _ _
                                end upd,
-                               argv,
-                               pos_args))
+                               argv))
               end)
       end%error).
 
@@ -335,30 +402,10 @@ Definition consume_help_or_named_arg
            (missing : string (* key *) -> parse_error)
            (wrong : string (* key *) -> string (* got *) -> string (* expected *) -> parse_error)
            (help : parse_error)
-  : parse_result ((keyed_spec_list_data named_args -> keyed_spec_list_data named_args) * list string (* remaining *) * list string (* accumulated positional args *))
+  : parse_result ((keyed_spec_list_data named_args -> keyed_spec_list_data named_args) * list string (* remaining *))
   := if arg_matches_key_list arg [short_key "h"; long_key "help"]
      then Error help
      else consume_named_arg arg argv named_args missing wrong.
-
-Fixpoint consume_named_args (fuel : nat)
-         (argv : list string)
-         (named_args : list (list key * spec * doc))
-         (missing : string (* key *) -> parse_error)
-         (wrong : string (* key *) -> string (* got *) -> string (* expected *) -> parse_error)
-         (help : parse_error)
-         (out_of_fuel : parse_error)
-         {struct fuel}
-  : parse_result ((keyed_spec_list_data named_args -> keyed_spec_list_data named_args) * list string (* remaining *))
-  := match argv, fuel with
-     | nil, _ => Success (id, nil)
-     | cons _ _, O => Error out_of_fuel
-     | cons arg argv, S fuel'
-       => (res <- consume_help_or_named_arg arg argv named_args missing wrong help;
-             let '(upd0, argv, pos_args) := res in
-             res <- @consume_named_args fuel' argv named_args missing wrong help out_of_fuel;
-               let '(upd_rest, argv) := res in
-               Success (fun st => upd_rest (upd0 st), pos_args ++ argv))
-     end%error.
 
 Definition consume_one_anon_arg (opt : bool) (argv : list string) (s : spec)
            (missing : parse_error)
@@ -378,45 +425,111 @@ Definition consume_one_anon_arg (opt : bool) (argv : list string) (s : spec)
           end
      end.
 
-Fixpoint consume_repeated_anon_arg (fuel : nat)
-         (argv : list string)
-         (s : spec)
-         (missing : parse_error)
-         (wrong : string (* got *) -> string (* expected *) -> parse_error)
-         (out_of_fuel : parse_error)
-         {struct fuel}
-  : parse_result (list (spec_data s) * list string (* remaining *))%type
-  := match argv, fuel with
-     | nil, _ => Success (nil, nil)
-     | cons _ _, O => Error out_of_fuel
-     | cons _ _, S fuel'
-       => (res <- consume_one_anon_arg false argv s missing wrong;
-             let '(v, argv) := res in
-             res <- @consume_repeated_anon_arg fuel' argv s missing wrong out_of_fuel;
-               let '(vs, argv) := res in
-               Success (v :: vs, argv))
-     end%error.
+Fixpoint Build_type_of_list_map {A}
+         {f l ls}
+         (v : l)
+         (vf : forall x, f x)
+         {struct ls}
+  : type_of_list l (@List.map A _ f ls)
+  := match ls with
+     | [] => v
+     | l' :: ls => @Build_type_of_list_map A f _ ls (v, vf _) vf
+     end.
 
-Fixpoint consume_anon_args
-         (opt : bool)
+Definition cons_spec_list_data {opt s1 s2 s3 ss}
+  : opt_spec_data opt s2 -> spec_list_data opt ss -> spec_list_data opt ((s1, s2, s3) :: ss)
+  := match ss with
+     | [] => fun v _ => v
+     | (_, _, _) :: _ => fun v vs => cons_type_of_list v vs
+     end.
+
+Definition empty_spec_list_data_opt
+           {anon_opt_args : list (string * spec * doc)}
+  : spec_list_data true anon_opt_args
+  := match anon_opt_args return spec_list_data true anon_opt_args with
+     | [] => tt
+     | (_, _, _) :: _ => Build_type_of_list_map (f:=fun '(_, _, _) => _) None (fun '(_, _, _) => None)
+     end.
+
+Definition empty_opt_repeated_arg {A B} {v : option (A * _ * B)}
+  : match v with
+    | Some (_, s0, _) => list (spec_data s0)
+    | None => unit
+    end
+  := match v with
+     | Some (_, _, _) => []
+     | None => tt
+     end.
+
+Fixpoint consume_args
+         (fuel : nat)
          (argv : list string)
-         (anon_args : list (string * spec * doc))
+         (s : arg_spec)
          (missing : string (* key *) -> parse_error)
          (wrong : string (* key *) -> string (* got *) -> string (* expected *) -> parse_error)
-         {struct anon_args}
-  : parse_result (spec_list_data opt anon_args * list string (* remaining *))%type
-  := match anon_args return parse_result (spec_list_data opt anon_args * list string)%type with
-     | nil => Success (tt, argv)
-     | cons (k, s, d) anon_args
-       => (res <- consume_one_anon_arg opt argv s (missing k) (wrong k);
-             let '(v, argv) := res in
-             rec <- consume_anon_args opt argv anon_args missing wrong;
-               Success (match anon_args return spec_list_data opt anon_args -> type_of_list (opt_spec_data opt s) (List.map (fun '(_, s0, _) => opt_spec_data opt s0) anon_args) with
-                        | nil => fun _ => v
-                        | cons (k', s', d') anon_args
-                          => fun vs
-                             => update_type_of_list _ _ _ (fun v' => (v, v')) vs
-                        end (fst rec), snd rec))
+         (too_many : list string (* remaining *) -> parse_error)
+         (internal_error : string (* msg *) -> parse_error)
+         (no_keyed_arg : list string (* unrecognized arguments *) -> parse_error)
+         (help : parse_error)
+         (out_of_fuel : parse_error)
+         {struct fuel}
+  : parse_result ((keyed_spec_list_data s.(named_args) -> keyed_spec_list_data s.(named_args)) * spec_list_data false s.(anon_args) * spec_list_data true s.(anon_opt_args) * (match s.(anon_opt_repeated_arg) with None => unit | Some (k, s, d) => list (spec_data s) end))%type
+  := let initial_len := List.length argv in
+     let do_recr s fuel' argv'
+         := if list_beq _ String.eqb argv argv'
+            then (* no progress *)
+              match argv' with
+              | [] => Error (internal_error "Encountered empty argument list when doing recursion in consume_args")
+              | arg :: _
+                => if String.startswith "-" arg
+                   then Error (no_keyed_arg [arg])
+                   else Error (too_many argv')
+              end
+            else
+              @consume_args fuel' argv' s missing wrong too_many internal_error no_keyed_arg help out_of_fuel in
+     let spec := s in
+     match argv, fuel with
+     | nil, _
+       => match s.(anon_args) as saa
+                return parse_result (_ * spec_list_data false saa * _ * _)%type
+          with
+          | [] => Success (fun data => data, tt, empty_spec_list_data_opt, empty_opt_repeated_arg)
+          | (k, s, d) :: _ => Error (missing k)
+          end
+     | cons _ _, O => Error out_of_fuel
+     | cons arg argv, S fuel'
+       => if String.startswith "-" arg
+          then (* named *)
+            (res <- consume_help_or_named_arg arg argv s.(named_args) missing wrong help;
+            let '(upd0, argv) := res in
+            res <- do_recr s fuel' argv;
+            let '(upd1, anon_data, anon_opt_data, anon_opt_repeated_data) := res in
+            Success (fun data => upd1 (upd0 data), anon_data, anon_opt_data, anon_opt_repeated_data))
+          else (* anonymous *)
+            let sna := s.(named_args) in
+            match s.(anon_args) as saa, s.(anon_opt_args) as saoa, s.(anon_opt_repeated_arg) as saora
+                  return parse_result ((keyed_spec_list_data s.(named_args) -> keyed_spec_list_data s.(named_args)) * spec_list_data false saa * spec_list_data true saoa * (match saora with None => unit | Some (k, s, d) => list (spec_data s) end))%type
+            with
+            | [], [], None => Error (too_many (arg :: argv))
+            | [], [], Some (k, s, d)
+              => (res <- consume_one_anon_arg false (arg :: argv) s (missing k) (wrong k);
+                 let '(v, argv) := res in
+                 res <- do_recr {| named_args := sna ; anon_args := [] ; anon_opt_args := [] ; anon_opt_repeated_arg := Some (k, s, d) |} fuel' argv;
+                 let '(upd, tt, tt, vs) := res in
+                 Success (upd, tt, tt, v :: vs))
+            | [], (k, s, d) :: saoa, saora
+              => (res <- consume_one_anon_arg true (arg :: argv) s (missing k) (wrong k);
+                 let '(v, argv) := res in
+                 res <- do_recr {| named_args := sna ; anon_args := [] ; anon_opt_args := saoa ; anon_opt_repeated_arg := saora |} fuel' argv;
+                 let '(upd, tt, vs, rest) := res in
+                 Success (upd, tt, cons_spec_list_data (opt:=true) v vs, rest))
+            | (k, s, d) :: saa, saoa, saora
+              => (res <- consume_one_anon_arg false (arg :: argv) s (missing k) (wrong k);
+                 let '(v, argv) := res in
+                 res <- do_recr {| named_args := sna ; anon_args := saa ; anon_opt_args := saoa ; anon_opt_repeated_arg := saora |} fuel' argv;
+                 let '(upd, vs, rest_opt, rest) := res in
+                 Success (upd, cons_spec_list_data (opt:=false) v vs, rest_opt, rest))
+            end
      end%error.
 
 Definition default_named_result {s} : spec_data_with_key s := nil.
@@ -440,34 +553,15 @@ Definition parse_argv (argv : list string) (arg_spec : arg_spec)
   := match argv with
      | nil => Error missing_prog_name
      | prog_name :: argv
-       => (res <- (consume_named_args (10 + (List.length argv)) argv (arg_spec.(named_args)) (missing prog_name) (wrong prog_name) (help prog_name) (out_of_fuel prog_name));
-             let '(upd, argv) := res in
-             res <- consume_anon_args false argv (arg_spec.(anon_args)) (missing prog_name) (wrong prog_name);
-               let '(anon_data, argv) := res in
-               res <- consume_anon_args true argv (arg_spec.(anon_opt_args)) (missing prog_name) (wrong prog_name);
-                 let '(anon_opt_data, argv) := res in
-                 res <- match anon_opt_repeated_arg arg_spec as r return
-                              parse_result
-                                (match r with
-                                 | None => unit
-                                 | Some (_, s, _) => list (spec_data s)
-                                 end
-                                 * list string)
-                        with
-                        | None => Success (tt, argv)
-                        | Some (k, s, d) => consume_repeated_anon_arg (10 + (List.length argv)) argv s (missing prog_name k) (wrong prog_name k) (out_of_fuel prog_name)
-                        end;
-                   let '(anon_repeated_opt_data, argv) := res in
-                   match argv with
-                   | nil => Success (upd default_named_results, anon_data, anon_opt_data, anon_repeated_opt_data)
-                   | _ => Error (too_many_args prog_name argv)
-                   end)
+       => (res <- consume_args (10 + (List.length argv)) argv arg_spec (missing prog_name) (wrong prog_name) (too_many_args prog_name) (internal_error prog_name) (no_keyed_arg prog_name) (help prog_name) (out_of_fuel prog_name);
+          let '(upd, anon_data, anon_opt_data, anon_opt_repeated_data) := res in
+          Success (upd default_named_results, anon_data, anon_opt_data, anon_opt_repeated_data))
      end%error.
 
 Definition is_real_error (e : parse_error) : bool := match e with help _ => false | _ => true end.
 
 Definition make_usage (prog_name : string) (spec : arg_spec) : string
-  := "USAGE:"
+  := "USAGE: "
        ++ prog_name ++ " [OPTS...] "
        ++ (String.concat
              " "
@@ -478,7 +572,7 @@ Definition make_usage (prog_name : string) (spec : arg_spec) : string
                    | None => nil
                    end)).
 
-Definition show_list_parse_error (spec : arg_spec) (err : parse_error) : list string
+Definition show_list_parse_error {should_block_indent : ShouldBlockIndent} (spec : arg_spec) (err : parse_error) : list string
   := let mk_usage prog_name err := (usage_string spec (err ++ [String.NewLine; make_usage prog_name spec]) ++ [String.NewLine])%list in
      match err with
      | help prog_name
@@ -490,6 +584,12 @@ Definition show_list_parse_error (spec : arg_spec) (err : parse_error) : list st
      | missing_prog_name => ["Empty argv" ++ String.NewLine]%string
      | too_many_args prog_name remaining
        => mk_usage prog_name [prog_name ++ ": unrecognized arguments: " ++ String.concat " " remaining]%string
+     | no_keyed_arg prog_name invalid_args
+       => mk_usage prog_name [prog_name ++ ": unrecognized keyed arguments: " ++ String.concat " " invalid_args]%string
+     | internal_error prog_name msg
+       => mk_usage prog_name [prog_name ++ ": Internal error (please report as a bug): " ++ msg]%string
      | out_of_fuel prog_name
        => mk_usage prog_name [prog_name ++ ": Internal fatal error while parsing command line arguments: Out of fuel (probably a bugged command line argument specification)"]%string
      end.
+
+Instance default_should_block_indent : ShouldBlockIndent := ArbitraryIndent.
